Midterm Friday 11/15
	Covers Ch. 3 & Ch. 4 in Holt

#### Review from Wednesday
$$
A=\begin{bmatrix}
1 & 0 & 4 & 2 \\
1 & 2 & 6 & 2 \\
2 & 0 & 8 & 8 \\
2 & 1 & 9 & 4
\end{bmatrix}\to^{GE}B=\begin{bmatrix}
1 & 0 & 4 & 2 \\
0 & 1 & 1 & 0 \\
0 & 0 & 0 & 4 \\
0 & 0 & 0 & 0
\end{bmatrix}
$$
Is this matrix invertible?
	3 pivots
	1 column w/o a pivot, so **not** invertible
Find basis for row space -> dim = # of pivots (3)
		for column space -> also # of pivots
		for null space -> dim = # of columns w/o pivot (1)

##### Basis for row space
$$
\left\{ \begin{bmatrix}
1&0&4&2
\end{bmatrix},\begin{bmatrix}
0&1&1&1
\end{bmatrix},\begin{bmatrix}
0&0&0&4
\end{bmatrix} \right\}
$$
Just took rows with pivots
**Find a relation**
	These rows are related with $R_{2}+3R_{1}-2R_{4}=0$
	(These are the steps performed in GE)
An alternative basis could be found by substituting rows from $A$ / $B$ or vice versa
$$
\left\{ \begin{bmatrix}
1&0&4&2
\end{bmatrix},\begin{bmatrix}
1 & 2 & 6 & 2
\end{bmatrix},\begin{bmatrix}
2 & 0 & 8 & 8
\end{bmatrix} \right\}
$$
##### Basis for column space
Find columns that have pivots after GE and use those columns from $A$
$$
\left\{ \begin{bmatrix}
1 \\
1 \\
2 \\
2
\end{bmatrix},\begin{bmatrix}
0 \\
2 \\
0 \\
1
\end{bmatrix},\begin{bmatrix}
2 \\
2 \\
8 \\
4
\end{bmatrix}
\right\}
$$
#### Basis for null space
$$
B=\begin{bmatrix}
1 & 0 & 4 & 2 \\
0 & 1 & 1 & 0 \\
0 & 0 & 0 & 4 \\
0 & 0 & 0 & 0
\end{bmatrix}
$$
Column 3 has no pivot, so free variable
Null space = $\left\{ x:Ax=0 \right\}=\left\{ x:Bx=0 \right\}$
	Row 3 -> $4x_{4}=0 : x_{4}=0$
	Row 2 -> $x_{2}+x_{3}=0 : x_{2}=-x_{3}=-s$
	Row 1 -> $x_{1}+4x_{3}+2x_{4}=0 : x_{1}=-4x_{3}=-4s$
$$
\begin{bmatrix}
-4s \\
-s \\
s \\
0
\end{bmatrix}\to \begin{bmatrix}
-4 \\
-1 \\
1 \\
0
\end{bmatrix}
$$
Basis for null space

#### Rank Nullity Theorem
dim(row space / column space) + dim(null space) = # of columns

## Change of Basis
Two basis of $\mathbb{R}^2$
	$\begin{bmatrix}1\\0\end{bmatrix},\begin{bmatrix}0\\1\end{bmatrix}$ standard basis
	$\begin{bmatrix}2\\1\end{bmatrix},\begin{bmatrix}-1\\1\end{bmatrix}$ new basis
Want to represent $\begin{bmatrix}3\\2\end{bmatrix}$ in both bases
	$\begin{bmatrix}3\\2\end{bmatrix}=3\begin{bmatrix}1\\0\end{bmatrix}+2\begin{bmatrix}0\\1\end{bmatrix}$ - pretty easy
	$\begin{bmatrix}3\\2\end{bmatrix}=a\begin{bmatrix}2\\1\end{bmatrix}+b\begin{bmatrix}-1\\1\end{bmatrix}=\begin{bmatrix}2&-1\\1&1\end{bmatrix}\begin{bmatrix}a\\b\end{bmatrix}$
		Many ways to solve this, but we're going to use the inverse
		$B^{-1}\begin{bmatrix}3\\2\end{bmatrix}=B^{-1}B\begin{bmatrix}a\\b\end{bmatrix}$
		$B^{-1}\begin{bmatrix}3\\2\end{bmatrix}=\begin{bmatrix}a\\b\end{bmatrix}$
		Finding the inverse
			$B^{-1}=\frac{1}{2(1)-(-1)(1)}\begin{bmatrix}1&1\\-1&2\end{bmatrix}$
		        $=\frac{1}{3}\begin{bmatrix}1&1\\-1&2\end{bmatrix}$
		$\begin{bmatrix}a\\b\end{bmatrix}=\frac{1}{3}\begin{bmatrix}1&1\\-1&2\end{bmatrix}=\begin{bmatrix}\left( \frac{5}{3}\right)\\\left( \frac{1}{3} \right)\end{bmatrix}$
		