Conditional statement, if-then

| $P$ | $Q$ | $P\to Q$ |
| --- | --- | -------- |
| T   | T   | T        |
| T   | F   | F        |
| F   | T   | T        |
| F   | F   | T        |
Implications are used in proofs
	If the originating axiom or theorem is true, then each individual implication must show that each step is true, leading to a chain that proves our claim

Converse
	Converse of $P\implies Q$ is $Q\implies P$
Equivalence:
	$(P\implies Q)\land(Q\implies P)$
Contrapositive:
	Contrapositive of $P\implies Q$ is $\neg Q\implies \neg P$
	These are equivalent $P\implies Q\equiv \neg Q\implies \neg P$
	